Fixed some merge conflicts.

ADTRefinement.v
@@ -1,4 +1,4 @@
-Require Import Common Computation ADT.
+Require Import Common Computation ADT Ensembles.
 
 Generalizable All Variables.
 Set Implicit Arguments.
@@ -19,32 +19,41 @@ Definition observerMethodSpec (Ty : Type) :=
 
 (** Every spec is trivially implementable using [Pick]. *)
 Section pick.
-  Variable model : Type.
+  Variable rep : Type.
   Variable mutatorMethodIndex : Type.
   Variable observerMethodIndex : Type.
-  Variable mutatorMethodSpecs : mutatorMethodIndex -> mutatorMethodSpec model.
-  Variable observerMethodSpecs : observerMethodIndex -> observerMethodSpec model.
+  Variable mutatorMethodSpecs : mutatorMethodIndex -> mutatorMethodSpec rep.
+  Variable observerMethodSpecs : observerMethodIndex -> observerMethodSpec rep.
 
-  Definition pickImpl : ADT :=
+  Local Obligation Tactic := econstructor; eauto.
+
+  Program Definition pickImpl : ADT :=
     {|
-      Model := model;
+      Rep := rep;
+      RepInv m := True;
       MutatorIndex := mutatorMethodIndex;
       ObserverIndex := observerMethodIndex;
       MutatorMethods idx :=
-        fun m x =>
-          { m' : model
-          | mutatorMethodSpecs idx m x m'}%comp;
+        fun r x =>
+          { r' : rep
+          | mutatorMethodSpecs idx r x r'}%comp;
       ObserverMethods idx :=
-        fun m n =>
+        fun r n =>
           { n' : nat
-          | observerMethodSpecs idx m n n'}%comp
+          | observerMethodSpecs idx r n n'}%comp
     |}.
+
 End pick.
 
 Section MethodRefinement.
-  Variables oldModel newModel : Type.
+  Variables oldRep newRep : Type.
+  (** Old and new representations **)
 
-  Variable abs : newModel -> Comp oldModel.
+  Variable oldRepInv : Ensemble oldRep.
+  Variable newRepInv : Ensemble newRep.
+  (** Old and new representation invariants **)
+
+  Variable abs : newRep -> Comp oldRep.
   (** Abstraction function *)
 
   (** Refinement of a mutator method: if we first do the new
@@ -53,17 +62,19 @@ Section MethodRefinement.
       following diagram commutes:
 <<
                    old mutator
-       old model --------------> old model
+       old rep --------------> old rep
           ↑                         ↑
       abs |                         | abs
           |                         |
-       new model --------------> new model
+       new rep --------------> new rep
                    new mutator
 >>  *)
+
   Definition refineMutator
-             (oldMutator : mutatorMethodType oldModel)
-             (newMutator : mutatorMethodType newModel)
+             (oldMutator : mutatorMethodType oldRep)
+             (newMutator : mutatorMethodType newRep)
     := forall new_state n,
+         newRepInv new_state ->
          refine (old_state <- abs new_state;
                  oldMutator old_state n)
                 (new_state' <- newMutator new_state n;
@@ -74,21 +85,42 @@ Section MethodRefinement.
       computation.  That is, the following diagram should commute:
 <<
                   old observer
-       old model --------------> ℕ
+       old rep --------------> ℕ
           ↑                      ∥
       abs |                      ∥ id
           |                      ∥
-       new model --------------> ℕ
+       new rep --------------> ℕ
                   new observer
 >>
    *)
   Definition refineObserver
-             (oldObserver : observerMethodType oldModel)
-             (newObserver : observerMethodType newModel)
+             (oldObserver : observerMethodType oldRep)
+             (newObserver : observerMethodType newRep)
     := forall new_state n,
+         newRepInv new_state ->
          refine (old_state <- abs new_state;
                  oldObserver old_state n)
                 (newObserver new_state n).
+
+  (**  Abstraction should preserve representation invariants:
+       The abstraction of a new representation that satisfies its
+       representation invariant should satisfy the old invariant.
+       Diagrammatically,
+
+  (Old RepInv holds)
+      old rep
+        ↑
+        | abs
+        |
+       new rep
+  (New RepInv holds)
+   **)
+
+  Definition absPreservesInv
+    := forall new_state,
+         newRepInv new_state ->
+         computational_inv oldRepInv (abs new_state).
+
 End MethodRefinement.
 
 (** We map from old indices to new indices because every method that
@@ -98,19 +130,24 @@ Inductive refineADT (A B : ADT) : Prop :=
 | refinesADT :
     forall abs mutatorMap observerMap,
       (forall idx, @refineMutator
-                     (Model A) (Model B) abs
+                     (Rep A) (Rep B)
+                     (RepInv B) abs
                      (MutatorMethods A idx)
                      (MutatorMethods B (mutatorMap idx)))
       -> (forall idx, @refineObserver
-                     (Model A) (Model B) abs
+                     (Rep A) (Rep B)
+                     (RepInv B) abs
                      (ObserverMethods A idx)
                      (ObserverMethods B (observerMap idx)))
+      -> (@absPreservesInv (Rep A) (Rep B)
+                 (RepInv A) (RepInv B) abs)
       -> refineADT A B.
 
 (** We should always just unfold [refineMutator] and [refineObserver]
     into [refine], so that we can rewrite with lemmas about [refine]. *)
 Arguments refineMutator / .
 Arguments refineObserver / .
+Arguments absPreservesInv / .
 
 Global Instance refineADT_PreOrder : PreOrder refineADT.
 Proof.
@@ -122,7 +159,8 @@ Proof.
       (observerMap := id);
       unfold id; simpl; intros;
       autorewrite with refine_monad;
-      reflexivity.
+      try reflexivity;
+      inversion_by computes_to_inv; subst; eauto.
   - intros x y z
            [abs mutMap obsMap mutH obsH]
            [abs' mutMap' obsMap' mutH' obsH'].
@@ -130,8 +168,20 @@ Proof.
     (abs := fun z => (z' <- abs' z; abs z')%comp)
     (mutatorMap := mutMap' ∘ mutMap)
     (observerMap := obsMap' ∘ obsMap);
-    unfold id, compose; simpl in *; intros;
-    interleave_autorewrite_refine_monad_with setoid_rewrite_hyp.
+    unfold id, compose; simpl in *; intros.
+    + autorewrite with refine_monad.
+      rewrite <- !refineEquiv_bind_bind, <- (mutH' _ _ _ H1).
+      rewrite !refineEquiv_bind_bind.
+      unfold refine; intros; inversion_by computes_to_inv.
+      econstructor; eauto.
+      eapply mutH; eauto.
+    + autorewrite with refine_monad.
+      rewrite <- !refineEquiv_bind_bind, <- (obsH' _ _ _ H1).
+      rewrite !refineEquiv_bind_bind.
+      unfold refine; intros; inversion_by computes_to_inv.
+      econstructor; eauto.
+      eapply obsH; eauto.
+    + inversion_by computes_to_inv; eauto.
 Qed.
 
 Add Parametric Relation : ADT refineADT
@@ -139,10 +189,11 @@ Add Parametric Relation : ADT refineADT
     transitivity proved by transitivity
       as refineADT_rel.
 
-Add Parametric Morphism model mutIdx obsIdx : (@Build_ADT model mutIdx obsIdx)
+Add Parametric Morphism rep repInv mutIdx obsIdx mutInv
+  : (fun ms os => @Build_ADT rep repInv mutIdx obsIdx ms os (mutInv ms))
   with signature
-  (pointwise_relation _ (@refineMutator _ _ (@Return _)))
-    ==> (pointwise_relation _ (@refineObserver _ _ (@Return _)))
+  (pointwise_relation _ (@refineMutator _ _ repInv (@Return _)))
+    ==> (pointwise_relation _ (@refineObserver _ _ repInv (@Return _)))
     ==> refineADT
     as refineADT_Build_ADT.
 Proof.
@@ -151,7 +202,7 @@ Proof.
   let B := match goal with |- refineADT ?A ?B => constr:(B) end in
   eapply (@refinesADT A B (@Return _) id id);
     unfold id, pointwise_relation in *; simpl in *; intros;
-    auto.
+    auto; inversion_by computes_to_inv; subst; eauto.
 Qed.
 
 (** If we had dependent setoid relations in [Type], then we could write
@@ -172,104 +223,655 @@ Qed.
 >>
 
     But, alas, Matthieu is still working on those.  So the rewrite
-    machinery won't work very well when we're switching models, and
+    machinery won't work very well when we're switching reps, and
     we'll instead have to use [etransitivity] and [apply] things. *)
 
-(* Given an abstraction function, we can transform the model of a pickImpl ADT. *)
+(* Given an abstraction function, we can transform the rep of a pickImpl ADT. *)
 
-Theorem refines_model_pickImpl
-        newModel oldModel
-        (abs : newModel -> oldModel)
-        MutatorIndex ObserverIndex
-        ObserverSpec MutatorSpec :
-  refineADT
-    (@pickImpl oldModel MutatorIndex ObserverIndex MutatorSpec ObserverSpec)
-    (@pickImpl newModel MutatorIndex ObserverIndex
-               (fun idx nm n nm' => MutatorSpec idx (abs nm) n (abs nm'))
-               (fun idx nm => ObserverSpec idx (abs nm))).
-Proof.
-  econstructor 1 with (abs := fun nm => Return (abs nm))
-                        (mutatorMap := @id MutatorIndex)
-                        (observerMap := @id ObserverIndex);
-  compute; intros; inversion_by computes_to_inv; subst; eauto.
-Qed.
+Section GeneralRefinements.
 
-(** We can cache an observer value by refining the model and the mutators. *)
+  Theorem refines_rep_pickImpl
+          newRep oldRep
+          (abs : newRep -> oldRep)
+          MutatorIndex ObserverIndex
+          ObserverSpec MutatorSpec :
+    refineADT
+      (@pickImpl oldRep MutatorIndex ObserverIndex MutatorSpec ObserverSpec)
+      (@pickImpl newRep MutatorIndex ObserverIndex
+                 (fun idx nm n nm' => MutatorSpec idx (abs nm) n (abs nm'))
+                 (fun idx nm => ObserverSpec idx (abs nm))).
+  Proof.
+    econstructor 1 with (abs := fun nm => Return (abs nm))
+                          (mutatorMap := @id MutatorIndex)
+                          (observerMap := @id ObserverIndex);
+    compute; intros; inversion_by computes_to_inv; subst; eauto.
+  Qed.
 
-Open Scope comp_scope.
+  Open Scope comp_scope.
 
-Theorem refines_cached_Observer adt
-        (ObserverIndex_eq : forall idx idx' : ObserverIndex adt,
-                               {idx = idx'} + {idx <> idx'})
-        (cachedIndex : ObserverIndex adt) (* Index of the Observer to Cache *)
-        (cached_func : Model adt -> nat -> nat)
-        (refines_cached : forall om n,
-                            refine (ObserverMethods adt cachedIndex om n)
-                                   (ret (cached_func om n)))
+  Section addCache.
 
-:
-  refineADT adt
-            {| Model := {om : (Model adt) * (nat -> nat) |
-                         forall n, refine (ObserverMethods adt cachedIndex (fst om) n) (ret (snd om n))};
-               MutatorIndex := MutatorIndex adt;
-               ObserverIndex := ObserverIndex adt;
-               ObserverMethods idx nm n :=
+  (* We can cache an observer value by refining the rep and the mutators. *)
+
+    Variable rep observerIndex : Type.
+    Variable ObserverIndex_eq : forall idx idx' : observerIndex,
+                                  {idx = idx'} + {idx <> idx'}.
+
+    Notation "x == y" := (ObserverIndex_eq x y) (at level 36).
+    Record cachedObservers :=
+      { origRep : rep;
+        observerCache : observerIndex -> option (nat -> nat)}.
+
+    (* A cache is well-formed if it refines all the observer methods
+     included in the cacheSet. *)
+    Definition ValidCache (cacheSet : observerIndex -> bool) ObserverMethods
+               (r : cachedObservers) :=
+      forall idx,
+        if cacheSet idx then
+          exists func,
+            observerCache r idx = Some func /\
+            forall n, refine (ObserverMethods idx r n) (ret (func n))
+        else
+          observerCache r idx = None.
+    Arguments ValidCache _ ObserverMethods r / .
+
+    Variable RepInv : Ensemble rep.
+    Definition AddValidCacheInv cacheSet ObserverMethods
+               (r : cachedObservers) :=
+      RepInv (origRep r) /\ ValidCache cacheSet ObserverMethods r.
+    Arguments AddValidCacheInv _ ObserverMethods r / .
+
+    (* A value is cached by applying a function to the representation
+      built by a mutator. *)
+    Definition ReplaceCachedObv
+               {MutatorIndex}
+               (MutatorMethods : MutatorIndex -> mutatorMethodType (cachedObservers))
+               (cachedIndex : observerIndex) (* Index of the Observer to Cache *)
+               (cachedFunc : rep -> nat -> nat)
+               idx m n :=
+      om <- MutatorMethods idx m n;
+      ret (Build_cachedObservers (origRep om)
+                                 (fun idx => if (idx == cachedIndex) then
+                                               Some (cachedFunc (origRep om))
+                                             else
+                                               observerCache om idx)).
+
+    Definition insertCachedSet cachedSet cachedIndex (idx : observerIndex) : bool :=
+      if (idx == cachedIndex) then
+        true
+      else
+        cachedSet idx.
+    Arguments insertCachedSet _ _ idx / .
+
+    (* Well-formed cached observer methods use the cache if it is available (naturally).
+     *)
+    Definition cachedObserverMethodsWF cachedObserverMethods :=
+      forall r idx f,
+        observerCache r idx = Some f ->
+        forall n,
+          refineEquiv (cachedObserverMethods idx r n) (ret (f n)).
+    Arguments cachedObserverMethodsWF _ / .
+
+    (* Well-formed cached observer methods will default to the original
+       observer methods for uncached indices.
+     *)
+    Definition cachedObserverMethodsWF' ObserverMethods cachedObserverMethods :=
+      forall r idx,
+        observerCache r idx = None ->
+        forall n : nat,
+          refine (A := nat) (ObserverMethods idx r n) (cachedObserverMethods idx r n).
+    Arguments cachedObserverMethodsWF' _ _ / .
+
+    (* Removing a cached value from a well-formed cache will produce
+       another well-formed cache value *)
+    Lemma RemoveValidCacheInv
+    : forall cachedSet cachedIndex ObserverMethods cachedObserverMethods r,
+        cachedObserverMethodsWF cachedObserverMethods ->
+        cachedObserverMethodsWF' ObserverMethods cachedObserverMethods ->
+        AddValidCacheInv cachedSet cachedObserverMethods r ->
+        AddValidCacheInv (fun idx =>
+                            if idx == cachedIndex
+                            then false
+                            else cachedSet idx)
+                         cachedObserverMethods
+    {| origRep := origRep r;
+       observerCache idx :=
+         if idx == cachedIndex then None else observerCache r idx |}.
+    Proof.
+      simpl; intros; intuition.
+      generalize (H3 idx); destruct (idx == cachedIndex);
+      find_if_inside; intuition; destruct_ex; intuition;
+      try (eexists; subst; split; eauto;
+           intros; generalize (H3 n); intros;
+           rewrite <- H; eauto; fail).
+      eexists; split; eauto; intros.
+      eapply H; simpl; eauto; find_if_inside; congruence.
+    Qed.
+    Hint Resolve RemoveValidCacheInv.
+
+    (* Removing a replaced cached value from a well-formed cache will produce
+       another well-formed cache value *)
+    Lemma ReplaceValidCacheInv
+    : forall cachedSet ObserverMethods cachedObserverMethods r
+        (refines_Observers : forall idx r n,
+                               refine (ObserverMethods idx r n) (cachedObserverMethods idx r n)),
+        AddValidCacheInv cachedSet cachedObserverMethods r ->
+        AddValidCacheInv cachedSet ObserverMethods r.
+    Proof.
+      simpl; intros; intuition.
+      generalize (H1 idx); find_if_inside; intuition; destruct_ex; intuition;
+      try (eexists; subst; split; eauto;
+           intros; generalize (H3 n); intros;
+           rewrite <- H; eauto; fail).
+    Qed.
+    Hint Resolve ReplaceValidCacheInv.
+
+    Lemma ReplaceCacheInv
+          {MutatorIndex cachedSet}
+          cachedObserverMethods
+          ObserverMethods MutatorMethods
+          (cachedIndex : observerIndex)
+          (cachedSetIndex : cachedSet cachedIndex = true)
+          cachedFunc
+          (refines_cached : forall r n,
+                              refine (cachedObserverMethods cachedIndex r n)
+                                     (ret (cachedFunc (origRep r) n)))
+          (refines_cached' : forall r idx f,
+                              observerCache r idx = Some f ->
+                              forall n,
+                                refineEquiv (ret (f n)) (cachedObserverMethods idx r n))
+          (refines_Observers : forall idx r n,
+                                 refine (ObserverMethods idx r n) (cachedObserverMethods idx r n))
+    : (forall idx  r n, AddValidCacheInv cachedSet ObserverMethods r ->
+                        computational_inv (AddValidCacheInv cachedSet ObserverMethods)
+                                          (MutatorMethods idx r n)) ->
+      forall (idx : MutatorIndex) r n,
+        AddValidCacheInv cachedSet cachedObserverMethods r ->
+        computational_inv
+          (AddValidCacheInv cachedSet cachedObserverMethods)
+          (ReplaceCachedObv MutatorMethods cachedIndex cachedFunc
+                            idx r n).
+    Proof.
+      unfold ReplaceCachedObv, computational_inv; intros.
+      apply_in_hyp computes_to_inv; destruct_ex; intuition;
+      apply_in_hyp computes_to_inv; destruct_ex; subst; simpl.
+      generalize (H idx r n (ReplaceValidCacheInv _ refines_Observers H0) _ H2); simpl; intuition.
+      generalize (H4 idx0); intros.
+      destruct (ObserverIndex_eq idx0 cachedIndex); subst; eauto.
+      rewrite cachedSetIndex in *|-*; eexists; split; eauto.
+      intros.
+      eapply refines_cached'; simpl; find_if_inside; congruence.
+      find_if_inside; destruct_ex; intuition; eauto.
+      eexists; intuition; eauto.
+      rewrite refines_cached'; subst; simpl; [reflexivity | eauto].
+      simpl; find_if_inside; subst; eauto.
+      congruence.
+    Qed.
+
+    Lemma AddCachedInv
+          {MutatorIndex cachedSet}
+          cachedObserverMethods
+          ObserverMethods MutatorMethods
+          (cachedIndex : observerIndex)
+          (cachedSetIndex : cachedSet cachedIndex = false)
+          cachedFunc
+          (refines_cached : forall r n,
+                              refine (cachedObserverMethods cachedIndex r n)
+                                     (ret (cachedFunc (origRep r) n)))
+          (refines_cached' : forall r idx f,
+                              observerCache r idx = Some f ->
+                              forall n,
+                                refineEquiv (ret (f n)) (cachedObserverMethods idx r n))
+          (refines_Observers : forall idx r n,
+                                 refine (ObserverMethods idx r n) (cachedObserverMethods idx r n))
+    : (forall idx  r n, AddValidCacheInv cachedSet ObserverMethods r ->
+                        computational_inv (AddValidCacheInv cachedSet ObserverMethods)
+                                          (MutatorMethods idx r n)) ->
+      forall (idx : MutatorIndex) r n,
+        AddValidCacheInv (insertCachedSet cachedSet cachedIndex) cachedObserverMethods r ->
+        computational_inv
+          (AddValidCacheInv (insertCachedSet cachedSet cachedIndex) cachedObserverMethods)
+          (ReplaceCachedObv MutatorMethods cachedIndex cachedFunc
+                            idx r n).
+    Proof.
+      unfold ReplaceCachedObv, computational_inv; intros.
+      apply_in_hyp computes_to_inv; destruct_ex; intuition;
+      apply_in_hyp computes_to_inv; destruct_ex; subst; simpl.
+      generalize (H idx r n (ReplaceValidCacheInv _ refines_Observers H0) _ H2); simpl; intuition.
+      generalize (H4 idx0); intros.
+      destruct (ObserverIndex_eq idx0 cachedIndex); subst; eauto.
+      rewrite cachedSetIndex in *|-*; eexists; split; eauto.
+      intros.
+      eapply refines_cached'; simpl; find_if_inside; congruence.
+      find_if_inside; destruct_ex; intuition; eauto.
+      eexists; intuition; eauto.
+      rewrite refines_cached'; subst; simpl; [reflexivity | eauto].
+      simpl; find_if_inside; subst; eauto.
+      congruence.
+    Qed.
+
+  End addCache.
+
+  Arguments ValidCache _ _ _ _ _ / .
+
+  Program Definition addCache adt : ADT :=
+    {| Rep := cachedObservers (Rep adt) (ObserverIndex adt);
+       RepInv := AddValidCacheInv (RepInv adt) (fun _ => false)
+                                  (fun idx r => ObserverMethods adt idx (origRep r)) ;
+       ObserverIndex := ObserverIndex adt;
+       MutatorIndex := MutatorIndex adt;
+       ObserverMethods idx r n :=
+         ObserverMethods adt idx (origRep r) n;
+       MutatorMethods idx r n :=
+         om <- MutatorMethods adt idx (origRep r) n;
+       ret {| origRep := om;
+              observerCache := fun _ => None |}
+    |}.
+  Next Obligation.
+    inversion_by computes_to_inv; subst; unfold AddValidCacheInv in *|-*; simpl; intuition.
+    eapply MutatorMethodsInv; eauto.
+  Defined.
+
+  Arguments addCache adt /.
+  Arguments Rep _ /.
+  Arguments AddValidCacheInv _ _ _ _ _ _ / .
+
+  Lemma refines_addCache : forall adt, refineADT adt (addCache adt).
+  Proof.
+    intros; destruct adt; simpl; econstructor 1 with
+                          (abs := fun m : @cachedObservers Rep ObserverIndex =>
+                                    ret (origRep m))
+                            (mutatorMap := @id MutatorIndex)
+                            (observerMap := @id ObserverIndex); simpl.
+    - intros; autorewrite with refine_monad; rewrite refineEquiv_under_bind with (g := @Return _);
+      intros; autorewrite with refine_monad; reflexivity.
+    - intros; autorewrite with refine_monad; unfold id; intuition.
+    - intros; inversion_by computes_to_inv; subst; intuition.
+  Qed.
+
+  Definition addCachedObserver
+          {Rep ObserverIndex MutatorIndex}
+          (cachedSet : ObserverIndex -> bool)
+          (repInv : Ensemble Rep)
+          ObserverMethods
+          (ObserverIndex_eq : forall idx idx' : ObserverIndex,
+                                   {idx = idx'} + {idx <> idx'})
+          (cachedIndex : ObserverIndex)
+          (cachedObserverMethods : ObserverIndex -> observerMethodType (cachedObservers Rep ObserverIndex))
+          (MutatorMethods : MutatorIndex -> mutatorMethodType (cachedObservers Rep ObserverIndex))
+          (MutatorMethodsInv :
+             forall idx r n, AddValidCacheInv repInv cachedSet ObserverMethods r ->
+                             computational_inv (AddValidCacheInv repInv cachedSet ObserverMethods)
+                                       (MutatorMethods idx r n))
+          cachedFunc
+          refines_cached
+          refines_Observers
+          cachedObserver_OK
+  : ADT :=
+    {| Rep := cachedObservers Rep ObserverIndex;
+       RepInv := AddValidCacheInv repInv (insertCachedSet _ cachedSet cachedIndex)
+                                  cachedObserverMethods;
+       ObserverIndex := ObserverIndex;
+       MutatorIndex := MutatorIndex;
+       ObserverMethods idx r n :=
+         match observerCache r idx with
+             Some func => ret (func n)
+           | _ => cachedObserverMethods idx r n
+         end;
+       MutatorMethods idx r n :=
+         ReplaceCachedObv ObserverIndex_eq MutatorMethods cachedIndex cachedFunc idx
+                          r n;
+       MutatorMethodsInv :=
+         @ReplaceCacheInv Rep ObserverIndex ObserverIndex_eq repInv
+                          MutatorIndex cachedSet cachedObserverMethods ObserverMethods
+                          MutatorMethods cachedIndex cachedFunc refines_cached refines_Observers
+                          cachedObserver_OK MutatorMethodsInv
+    |}.
+
+  Lemma refine_under_bind X Y (P : Ensemble X) (f g : X -> Comp Y) x y
+        (compInv : computational_inv P x)
+        (compInv' : computational_inv P y)
+        (eqv_f_g : forall x, P x -> refine (f x) (g x))
+        (refine_x_y : refine x y)
+  : refine (Bind x f)
+           (Bind y g).
+  Proof.
+    unfold refine; intros.
+    inversion_by computes_to_inv; econstructor; eauto.
+    eapply eqv_f_g; eauto.
+  Qed.
+
+  Print Implicit addCachedObserver.
+
+  Lemma refine_ret_eq : forall (A : Type) (a a' : A),
+                          refine (ret a) (ret a') -> a = a'.
+  Proof.
+    unfold refine; intros; generalize (H a' (ReturnComputes _)).
+    intros; inversion_by computes_to_inv; auto.
+  Qed.
+
+  Theorem refines_addCachedObserver
+          {Rep ObserverIndex MutatorIndex}
+          cachedSet
+          (repInv : Ensemble Rep)
+          ObserverMethods
+          cachedObserverMethods
+          MutatorMethods
+          (MutatorMethodsInv :
+             forall (idx : MutatorIndex) (r : cachedObservers Rep ObserverIndex)
+                    (n : nat),
+               AddValidCacheInv cachedSet ObserverMethods repInv r ->
+               computational_inv (AddValidCacheInv cachedSet ObserverMethods repInv)
+                                 (MutatorMethods idx r n))
+          ObserverIndex_eq
+          cachedIndex
+          cachedFunc
+          refines_cached
+          refines_cached'
+          refines_Observers
+  : cachedSet cachedIndex = true ->
+    refineADT {| Rep := cachedObservers Rep ObserverIndex;
+                 RepInv := AddValidCacheInv cachedSet ObserverMethods repInv;
+                  ObserverIndex := ObserverIndex;
+                  MutatorIndex := MutatorIndex;
+                  ObserverMethods := cachedObserverMethods;
+                  MutatorMethods := MutatorMethods;
+                  MutatorMethodsInv := MutatorMethodsInv
+               |}
+              (addCachedObserver ObserverIndex_eq cachedIndex
+                                 cachedObserverMethods MutatorMethods
+                                 MutatorMethodsInv cachedFunc
+                                 refines_cached refines_cached' refines_Observers).
+  Proof.
+    idtac.
+    unfold addCachedObserver.
+    econstructor 1 with (abs := fun nm : cachedObservers Rep ObserverIndex =>
+                                  if (cachedSet cachedIndex) then
+                                    ret nm
+                                  else
+                                    ret {| origRep := origRep nm;
+                                           observerCache idx :=
+                                             if ObserverIndex_eq idx cachedIndex then
+                                               None
+                                             else observerCache nm idx |})
+                          (mutatorMap := @id MutatorIndex)
+                          (observerMap := @id ObserverIndex); simpl.
+    - intros; rewrite H; autorewrite with refine_monad; unfold ReplaceCachedObv.
+      unfold insertCachedSet in H0.
+      unfold AddValidCacheInv in MutatorMethodsInv.
+      rewrite <- refineEquiv_unit_bind; apply refine_under_bind with
+                                        (P := AddValidCacheInv cachedSet ObserverMethods repInv); intros.
+      + eapply MutatorMethodsInv; simpl; intuition.
+        generalize (H2 idx0).
+        destruct (ObserverIndex_eq idx0 cachedIndex); intros; eauto.
+        subst; rewrite H.
+        destruct H0 as [func [func_eq refine_func] ]; eexists; split; eauto.
+        intros; rewrite refines_Observers; eauto.
+        find_if_inside; destruct_ex; eexists; intuition; eauto.
+        rewrite refines_Observers; eauto.
+      + eapply MutatorMethodsInv; simpl; intuition.
+        generalize (H2 idx0).
+        destruct (ObserverIndex_eq idx0 cachedIndex); intros; eauto.
+        subst; rewrite H.
+        destruct H0 as [func [func_eq refine_func] ]; eexists; split; eauto.
+        intros; rewrite refines_Observers; eauto.
+        find_if_inside; destruct_ex; eexists; intuition; eauto.
+        rewrite refines_Observers; eauto.
+      + simpl in H1; intuition; destruct x; simpl in *|-*.
+        assert (observerCache0 = fun idx0 =>
+                                   if ObserverIndex_eq idx0 cachedIndex
+                                   then Some (cachedFunc origRep0)
+                                   else observerCache0 idx0).
+        * apply functional_extensionality; intros.
+          find_if_inside; subst; eauto.
+          generalize (H4 cachedIndex); rewrite H; intros; destruct_ex;
+          intuition.
+          rewrite H5.
+          apply f_equal; apply functional_extensionality; intros.
+          generalize (refines_cached' {| origRep := origRep0; observerCache := observerCache0 |} _ _ H5 x0); intros.
+          destruct H1.
+          rewrite refines_cached in H1.
+          rewrite (refine_ret_eq H1); auto.
+        * rewrite H1 at 1; reflexivity.
+      + reflexivity.
+    - intros; rewrite H; autorewrite with refine_monad;
+      intuition; unfold insertCachedSet in H2.
+      generalize (H2 idx); simpl.
+      destruct (ObserverIndex_eq idx cachedIndex); intros; eauto.
+      subst.
+      unfold id; destruct H0 as [func [func_eq refine_func] ]; rewrite func_eq;
+      eauto.
+      generalize (refines_cached' new_state idx).
+      unfold id; destruct (observerCache new_state idx).
+      intros; rewrite H3; eauto; reflexivity.
+      intros; reflexivity.
+    - rewrite H; intros; inversion_by computes_to_inv; subst; intuition.
+      unfold insertCachedSet in H3; generalize (H3 idx); simpl.
+      destruct (ObserverIndex_eq idx cachedIndex); intros; eauto;
+      subst.
+      rewrite H; destruct_ex; eexists; intuition; eauto.
+      rewrite refines_Observers; eauto.
+      destruct (cachedSet idx); eauto.
+      destruct_ex; eexists; intuition; eauto.
+      rewrite refines_Observers; eauto.
+  Qed.
+
+  Theorem refines_addCachedObserver'
+          {Rep ObserverIndex MutatorIndex}
+          cachedSet
+          (repInv : Ensemble Rep)
+          ObserverMethods
+          cachedObserverMethods
+          MutatorMethods
+          (MutatorMethodsInv :
+             forall (idx : MutatorIndex) (r : cachedObservers Rep ObserverIndex)
+                    (n : nat),
+               AddValidCacheInv cachedSet ObserverMethods repInv r ->
+               computational_inv (AddValidCacheInv cachedSet ObserverMethods repInv)
+                                 (MutatorMethods idx r n))
+          ObserverIndex_eq
+          cachedIndex
+          cachedFunc
+          refines_cached
+          refines_cached'
+          refines_Observers
+  : cachedSet cachedIndex = false ->
+    refineADT {| Rep := cachedObservers Rep ObserverIndex;
+                 RepInv := AddValidCacheInv cachedSet ObserverMethods repInv;
+                  ObserverIndex := ObserverIndex;
+                  MutatorIndex := MutatorIndex;
+                  ObserverMethods := cachedObserverMethods;
+                  MutatorMethods := MutatorMethods;
+                  MutatorMethodsInv := MutatorMethodsInv
+               |}
+              (addCachedObserver ObserverIndex_eq cachedIndex
+                                 cachedObserverMethods MutatorMethods
+                                 MutatorMethodsInv cachedFunc
+                                 refines_cached refines_cached' refines_Observers).
+  Proof.
+    idtac.
+    unfold addCachedObserver.
+    econstructor 1 with (abs := fun nm : cachedObservers Rep ObserverIndex =>
+                                  if (cachedSet cachedIndex) then
+                                    ret nm
+                                  else
+                                    ret {| origRep := origRep nm;
+                                           observerCache idx :=
+                                             if ObserverIndex_eq idx cachedIndex then
+                                               None
+                                             else observerCache nm idx |})
+                          (mutatorMap := @id MutatorIndex)
+                          (observerMap := @id ObserverIndex); simpl.
+    - intros; rewrite H; autorewrite with refine_monad; unfold ReplaceCachedObv.
+      unfold insertCachedSet in H0.
+      unfold AddValidCacheInv in MutatorMethodsInv.
+      autorewrite with refine_monad.
+      generalize MutatorMethodsInv; simpl.
+      rewrite <- refineEquiv_unit_bind. apply refine_under_bind with
+                                        (P := AddValidCacheInv cachedSet ObserverMethods repInv); intros.
+      + eapply MutatorMethodsInv; simpl; intuition.
+        generalize (H2 idx0).
+        destruct (ObserverIndex_eq idx0 cachedIndex); intros; eauto.
+        subst; rewrite H.
+        destruct H0 as [func [func_eq refine_func] ]; eexists; split; eauto.
+        intros; rewrite refines_Observers; eauto.
+        find_if_inside; destruct_ex; eexists; intuition; eauto.
+        rewrite refines_Observers; eauto.
+      + simpl in H1; intuition; destruct x; simpl in *|-*.
+        assert (observerCache0 = fun idx0 =>
+                                   if ObserverIndex_eq idx0 cachedIndex
+                                   then Some (cachedFunc origRep0)
+                                   else observerCache0 idx0).
+        * apply functional_extensionality; intros.
+          find_if_inside; subst; eauto.
+          generalize (H4 cachedIndex); rewrite H; intros; destruct_ex;
+          intuition.
+          rewrite H5.
+          apply f_equal; apply functional_extensionality; intros.
+          generalize (refines_cached' {| origRep := origRep0; observerCache := observerCache0 |} _ _ H5 x0); intros.
+          destruct H1.
+          rewrite refines_cached in H1.
+          rewrite (refine_ret_eq H1); auto.
+        * rewrite H1 at 1; reflexivity.
+    - intros; rewrite H; autorewrite with refine_monad;
+      intuition; unfold insertCachedSet in H2.
+      generalize (H2 idx); simpl.
+      destruct (ObserverIndex_eq idx cachedIndex); intros; eauto.
+      subst.
+      unfold id; destruct H0 as [func [func_eq refine_func] ]; rewrite func_eq;
+      eauto.
+      generalize (refines_cached' new_state idx).
+      unfold id; destruct (observerCache new_state idx).
+      intros; rewrite H3; eauto; reflexivity.
+      intros; reflexivity.
+    - rewrite H; intros; inversion_by computes_to_inv; subst; intuition.
+      unfold insertCachedSet in H3; generalize (H3 idx); simpl.
+      destruct (ObserverIndex_eq idx cachedIndex); intros; eauto;
+      subst.
+      rewrite H; destruct_ex; eexists; intuition; eauto.
+      rewrite refines_Observers; eauto.
+      destruct (cachedSet idx); eauto.
+      destruct_ex; eexists; intuition; eauto.
+      rewrite refines_Observers; eauto.
+  Qed.
+
+rewrite func
+
+eexists; split; eauto.
+      intros; rewrite refines_Observers; eauto.
+      find_if_inside; destruct_ex; eexists; intuition; eauto.
+        rewrite refines_Observers; eauto.
+      unfold insertCachedSet in H0.
+      unfold insertO
+      destruct (observerCache new_state (id idx)).
+      simpl.
+      case (cachedSet cachedIndex).
+      find_if_inside; autorewrite with refine_monad.
+
+      generalize (MutatorMethodsInv idx _ n H); simpl; intros.
+      unfold refine; intros v H3; apply computes_to_inv in H3; destruct_ex; intuition.
+      apply computes_to_inv in H4; subst.
+      destruct (H0 _ H); destruct x; simpl in *.
+      assert (observerCache0 = fun idx0 : ObserverIndex =>
+                      if ObserverIndex_eq idx0 cachedIndex
+                      then Some (cachedFunc origRep0)
+                      else observerCache0 idx0).
+      apply functional_extensionality; intros.
+
+
+      setoid_replace (fun idx0 : ObserverIndex =>
+                        if ObserverIndex_eq idx0 cachedIndex
+                      then Some (cachedFunc origRep0)
+                      else observerCache0 idx0) with observerCache0.
+
+
+
+      rewrite <- refineEquiv_unit_bind; apply refine_under_bind; intros.
+      destruct x; simpl.
+      apply
+      rewrite (proj1 (refineEquiv_under_bind _ (@Return _) _ _)); autorewrite with refine_monad.
+      reflexivity.
+      intuition; split; simpl.
+      assert (observerCache0 = fun idx0 : ObserverIndex =>
+                         if ObserverIndex_eq idx0 cachedIndex
+                         then Some (cachedFunc origRep0)
+                         else observerCache0 idx0).
+      apply functional_extensionality; intros; find_if_inside.
+
+
+      intros; autorewrite with refine_monad.
+
+
+  Theorem refines_cached_Observer adt
+          (ObserverIndex_eq : forall idx idx' : ObserverIndex adt,
+                                {idx = idx'} + {idx <> idx'})
+          (cachedIndex : ObserverIndex adt) (* Index of the Observer to Cache *)
+          (cached_func : Rep adt -> nat -> nat)
+          (refines_cached : forall om n,
+                              refine (ObserverMethods adt cachedIndex om n)
+                                     (ret (cached_func om n)))
+
+  :
+    refineADT adt
+              {| Rep := {om : (Rep adt) * (nat -> nat) |
+                           forall n, refine (ObserverMethods adt cachedIndex (fst om) n) (ret (snd om n))};
+                 ObserverMethods idx nm n :=
                    if (ObserverIndex_eq idx cachedIndex) then
                      ret ((snd (proj1_sig nm)) n)
                    else
                      ObserverMethods adt idx (fst (proj1_sig nm)) n;
                  MutatorMethods idx nm n :=
-                   origModel <- (MutatorMethods adt idx (fst (proj1_sig nm)) n);
-                     ret (exist
-                            (fun om => forall n, refine (ObserverMethods adt cachedIndex (fst om) n) (ret (snd om n)))
-                            (origModel, cached_func origModel)
-                            (refines_cached origModel))|}.
-Proof.
-  destruct adt;
-  econstructor 1 with
-  (abs := fun om : {om | forall n, refine (ObserverMethods cachedIndex (fst om) n) (ret (snd om n))} =>
-            ret (fst (proj1_sig om)))
-    (mutatorMap := @id MutatorIndex)
-    (observerMap := @id ObserverIndex); simpl; intros.
-  - autorewrite with refine_monad; rewrite refineEquiv_under_bind with (g := @Return _);
-    intros; autorewrite with refine_monad; reflexivity.
-  - autorewrite with refine_monad; find_if_inside;
-    [ destruct new_state; subst; auto
+                   origRep <- (MutatorMethods adt idx (fst (proj1_sig nm)) n);
+                 ret (exist
+                        (fun om => forall n, refine (ObserverMethods adt cachedIndex (fst om) n) (ret (snd om n)))
+                        (origRep, cached_func origRep)
+                        (refines_cached origRep))|}.
+  Proof.
+    destruct adt;
+    econstructor 1 with
+    (abs := fun om : {om | forall n, refine (ObserverMethods cachedIndex (fst om) n) (ret (snd om n))} =>
+              ret (fst (proj1_sig om)))
+      (mutatorMap := @id MutatorIndex)
+      (observerMap := @id ObserverIndex); simpl; intros.
+    - autorewrite with refine_monad; rewrite refineEquiv_under_bind with (g := @Return _);
+      intros; autorewrite with refine_monad; reflexivity.
+    - autorewrite with refine_monad; find_if_inside;
+      [ destruct new_state; subst; auto
       | reflexivity].
-Qed.
+  Qed.
 
-Theorem refines_cached_computational_Observer adt
-        (ObserverIndex_eq : forall idx idx' : ObserverIndex adt,
-                               {idx = idx'} + {idx <> idx'})
-        (cachedIndex : ObserverIndex adt) (* Index of the Observer to Cache *)
-        (computational_Index : forall om n, is_computational (ObserverMethods adt cachedIndex om n))
-:
-  refineADT adt
-  {| Model := {om : (Model adt) * (nat -> nat) |
-               forall n, refine (ObserverMethods adt cachedIndex (fst om) n) (ret (snd om n))};
-     MutatorIndex := MutatorIndex adt;
-     ObserverIndex := ObserverIndex adt;
-     ObserverMethods idx nm n :=
-       if (ObserverIndex_eq idx cachedIndex) then
+  Theorem refines_cached_computational_Observer adt
+          (ObserverIndex_eq : forall idx idx' : ObserverIndex adt,
+                                {idx = idx'} + {idx <> idx'})
+          (cachedIndex : ObserverIndex adt) (* Index of the Observer to Cache *)
+          (computational_Index : forall om n, is_computational (ObserverMethods adt cachedIndex om n))
+  :
+    refineADT adt
+              {| Rep := {om : (Rep adt) * (nat -> nat) |
+                           forall n, refine (ObserverMethods adt cachedIndex (fst om) n) (ret (snd om n))};
+                 MutatorIndex := MutatorIndex adt;
+                 ObserverIndex := ObserverIndex adt;
+                 ObserverMethods idx nm n :=
+                   if (ObserverIndex_eq idx cachedIndex) then
                      ret ((snd (proj1_sig nm)) n)
-       else
-         ObserverMethods adt idx (fst (proj1_sig nm)) n;
-     MutatorMethods idx nm n :=
-                   origModel <- (MutatorMethods adt idx (fst (proj1_sig nm)) n);
-     ret (exist
-            (fun om => forall n, refine (ObserverMethods adt cachedIndex (fst om) n) (ret (snd om n)))
-            (origModel, fun n => is_computational_val (computational_Index origModel n))
-            (fun n => proj1 (refineEquiv_is_computational (computational_Index origModel n)))) |}.
-Proof.
-  apply refines_cached_Observer.
-Qed.
+                   else
+                     ObserverMethods adt idx (fst (proj1_sig nm)) n;
+                 MutatorMethods idx nm n :=
+                   origRep <- (MutatorMethods adt idx (fst (proj1_sig nm)) n);
+                 ret (exist
+                        (fun om => forall n, refine (ObserverMethods adt cachedIndex (fst om) n) (ret (snd om n)))
+                        (origRep, fun n => proj1_sig (is_computational_val (computational_Index origRep n)))
+                        (fun n => refine_is_computational (computational_Index origRep n))) |}.
+  Proof.
+    apply refines_cached_Observer.
+  Qed.
 
 (** If you mutate and then observe, you can do it before or after
     refinement.  I'm not actually sure this isn't obvious.  *)
 
 Lemma ADTRefinementOk
       (old new : ADT)
-      (new_initial_value : Comp (Model new))
+      (new_initial_value : Comp (Rep new))
       abs mutatorMap observerMap H H'
       (ref : refineADT old new
        := @refinesADT old new abs mutatorMap observerMap H H')
