ADT.v
@@ -19,19 +19,28 @@ Definition observerMethodType (Ty : Type) :=
 (** Interface of an ADT *)
 Record ADT :=
   {
-    Model : Type;
+    Rep : Type;
     (** The way we model state mathematically *)
- 
+
+    RepInv : Rep -> Prop;
+    (** Invariants on the Representation **)
+
     MutatorIndex : Type;
     (** The index set of mutators *)
 
     ObserverIndex : Type;
     (** The index set of observers *)
 
-    MutatorMethods : MutatorIndex -> mutatorMethodType Model;
+    MutatorMethods : MutatorIndex -> mutatorMethodType Rep;
     (** Mutator method implementations *)
 
-    ObserverMethods : ObserverIndex -> observerMethodType Model
+    ObserverMethods : ObserverIndex -> observerMethodType Rep;
     (** Observer method implementations *)
-  }.
 
+    MutatorMethodsInv : forall idx r n, RepInv r -> computational_inv RepInv (MutatorMethods idx r n)
+    (** Mutator methods maintain Representation Invariants **)
+
+    (** We probably want some sort of observer method specs as well.
+     That can wait until the next iteration of the ADT with arbitrary signatures. **)
+
+  }.
